fragmented.v
@@ -1,0 +1,117 @@
+(* Copyright (c) 2012-2013, Robbert Krebbers. *)
+(* This file is distributed under the terms of the BSD license. *)
+(** This file defines a type [frag A] to represent symbolic fragments of a
+data type [A]. The representation of [x : A] as a list of [n] fragments is:
+"frag 0 of x", ..., "frag n of x".  We provide functions to ``split'' an
+element of type [A] into fragments, and to go back. Fragments are used to
+describe abstract fragments of pointers so as to encode and decode pointers as
+bytes in the file [pointers]. *)
+Require Export numbers list.
+
+Record frag (A : Type) := Frag { frag_item : A; frag_index : nat }.
+Add Printing Constructor frag.
+Arguments Frag {_} _ _.
+Arguments frag_item {_} _.
+Arguments frag_index {_} _.
+
+Section fragmented.
+Context {A : Type} `{∀ x y : A, Decision (x = y)}.
+Context (len : nat) {len_pos : PropHolds (len ≠ 0)}.
+
+Global Instance frag_eq_dec (s1 s2 : frag A) : Decision (s1 = s2).
+Proof. solve_decision. Defined.
+
+Inductive fragmented (x : A) : nat → list (frag A) → Prop :=
+  | fragmented_nil : fragmented x len []
+  | fragmented_cons i xss :
+     fragmented x (S i) xss → fragmented x i (Frag x i :: xss).
+
+Global Instance fragmented_dec x : ∀ i xss, Decision (fragmented x i xss).
+Proof.
+ refine (
+  fix go i xss :=
+  match xss with
+  | [] => cast_if (decide_rel (=) len i)
+  | Frag y j :: pss =>
+     cast_if_and3 (decide_rel (=) i j) (decide_rel (=) x y) (go (S j) pss)
+  end); clear go len_pos; abstract (simplify_equality;
+      first [by constructor | by inversion 1]).
+Defined.
+
+Lemma fragmented_length x i xss : fragmented x i xss → i + length xss = len.
+Proof. induction 1; simpl; lia. Qed.
+Lemma fragmented_seq x i xss :
+  fragmented x i xss → Frag x <$> seq i (length xss) = xss.
+Proof. induction 1; simpl; by f_equal. Qed.
+
+Lemma fragmented_alt x i xss :
+  fragmented x i xss ↔
+    i + length xss = len ∧ xss = Frag x <$> seq i (length xss).
+Proof.
+  split; [intros Hvalid; split |].
+  * by apply fragmented_length with x.
+  * by rewrite fragmented_seq.
+  * intros [Hi Hxss]. rewrite Hxss. clear Hxss. revert i Hi.
+    induction (length xss); simpl; intros i.
+    + rewrite Nat.add_0_r. intros; subst. constructor.
+    + constructor. apply IHn. lia.
+Qed.
+
+Definition to_frags (x : A) : list (frag A) := Frag x <$> seq 0 len.
+Definition of_frags (xss : list (frag A)) : option A :=
+  match xss with
+  | Frag x 0 :: xss => guard (fragmented x 1 xss); Some x
+  | _ => None
+  end.
+
+Lemma to_frags_fragmented x : fragmented x 0 (to_frags x).
+Proof.
+  unfold to_frags. apply fragmented_alt. by rewrite fmap_length, seq_length.
+Qed.
+Lemma to_frags_length x : length (to_frags x) = len.
+Proof.
+  unfold to_frags. rewrite <-(plus_O_n (length _)).
+  apply fragmented_length with x, to_frags_fragmented.
+Qed.
+
+Lemma of_to_frags x xss : of_frags xss = Some x ↔ to_frags x = xss.
+Proof.
+  unfold of_frags, to_frags, PropHolds in *.
+  destruct len as [|n] eqn:?; simpl; [lia |]. split; intros Hss.
+  * destruct xss as [|[y [|?]] xss]; simplify_option_equality.
+    replace n with (length xss).
+    + by rewrite fragmented_seq.
+    + pose proof (fragmented_length x 1 xss). intuition lia.
+  * simplify_option_equality; [done |].
+    match goal with H : ¬fragmented _ _ _ |- _ => destruct H end;
+      apply fragmented_alt.
+    rewrite fmap_length, seq_length. intuition lia.
+Qed.
+Lemma of_to_frags_1 x xss : of_frags xss = Some x → to_frags x = xss.
+Proof. by apply of_to_frags. Qed.
+Lemma of_to_frags_2 x : of_frags (to_frags x) = Some x.
+Proof. by apply of_to_frags. Qed.
+
+Global Instance to_frags_inj: Injective (=) (=) to_frags.
+Proof.
+  intros x y. generalize (eq_refl (to_frags y)).
+  rewrite <-!of_to_frags. congruence.
+Qed.
+
+Lemma Forall_to_frags (P : frag A → Prop) x :
+  (∀ i, i < len → P (Frag x i)) → Forall P (to_frags x).
+Proof.
+  unfold to_frags. intros. apply Forall_fmap, Forall_seq; auto with lia.
+Qed.
+Lemma Forall_of_frags (P : frag A → Prop) x xss i :
+  of_frags xss = Some x → i < len → Forall P xss → P (Frag x i).
+Proof.
+  revert xss i. assert (∀ i xss,
+    S i < len → fragmented x 1 xss → Forall P xss → P (Frag x (S i))).
+  { intros i xss ?. rewrite fragmented_alt. intros [? Hxss].
+    rewrite Hxss. rewrite Forall_fmap, Forall_seq.
+    intros Hx. apply Hx; auto with lia. }
+  unfold of_frags. intros. destruct xss as [|[? [|?]]], i;
+    simplify_option_equality; decompose_Forall; eauto.
+Qed.
+End fragmented.
